Final

Naturals.v
@@ -2,145 +2,63 @@
 Require Import Basics.
 Require Import Reduction.
 
-Fixpoint church_nat_aux (n: nat): term :=
+Fixpoint encode_aux (n: nat): term :=
   match n with
   | 0 => #0
-  | S n' => $ (#1) (church_nat_aux n')
+  | S n' => $ (#1) (encode_aux n')
   end
 .
 
-
-
-(* Module test_church_nat.
-  Compute church_nat 0.
-  Compute church_nat 1.
-  Compute church_nat 2.
+(* Module test_encode.
+  Compute encode 0.
+  Compute encode 1.
+  Compute encode 2.
   (* etc. *)
-End test_church_nat. *)
+End test_encode. *)
 
 (* Church encoding of a given natural *)
-Definition church_nat (n: nat): term :=
-  \\(church_nat_aux n)
+Definition encode (n: nat): term :=
+  \\(encode_aux n)
 .
-
-Record term_nat := {
-  t: term;
-  (* We are strict: a Church numeral has to be in normal form to be considered as one, hence = instead of ==: *)
-  n: exists (n: nat), t = church_nat n;
-}.
-
-Program Definition church_nat' (n: nat): term_nat := {|
-  t := church_nat n;
-|}.
-
-Next Obligation.
-  now exists n0.
-Qed.
 
 
 (* TODO fix this notation? *)
-Definition church_succ: term :=
+Definition succ: term :=
   \\\ $ (#1) ($ ($ (#2) (#1)) (#0))
 .
 
-(* apply CTrans with (x' := p);
-[ apply CStep; unfold beta_step; simpl; now left | ]. *)
-
-(* Lemma replace_lemma (n: nat): $ (\ (\ church_nat_aux n)) (# 1) == \ church_nat_aux n.
-Proof.
-  induction n.
-  (* TODO do base case! *)
-  Focus 2.
-  unfold church_nat_aux; fold church_nat_aux. *)
-
-
-Fixpoint abstractionless (p: term): Prop :=
-  match p with
-  | #n => True
-  | \q => False
-  | $ q r => (abstractionless q) /\ (abstractionless r)
-  end
-.
 Require Import Coq.Arith.EqNat.
 
 Compute beta $ (\ #23) (#0) PRoot.
 
-(* Lemma eta_lemma (p: term) (_: abstractionless p) (n: nat): replace p (#n) n = p.
-Proof.
-  induction p.
-  - unfold replace.
-    destruct (EqNat.eq_nat_decide n n0).
-    + f_equal.
-      unfold increase_free_variables.
-      destruct (Compare_dec.le_lt_dec 0 n).
-      * 
-      now apply eq_nat_eq.
-    + reflexivity.
-  - contradict H.
-  - unfold replace; fold replace.
-    destruct H.
-    f_equal.
-    + now apply IHp1.
-    + now apply IHp2.
-Qed.
+Compute let n:=2 in (increase_free_variables (encode_aux n) 2 2, encode_aux n).
 
-
-Lemma eta (p: term) (_: abstractionless p): $ (\ p) (#0) == p.
-Proof.
-  apply CStep.
-  exists PRoot.
-  unfold beta.
-  f_equal.
-  now apply eta_lemma.
-Qed.
-
-Lemma eta1 (p: term) (_: abstractionless p): $ (\\ p) (#1) == \p.
-Proof.
-  apply CStep.
-  exists PRoot.
-  unfold beta.
-  unfold replace; fold replace.
-  f_equal.
-  f_equal.
-  now apply eta_lemma.
-Qed.
-
-Lemma abstractionless_church_nat_aux (n: nat): abstractionless (church_nat_aux n).
-Proof.
-  induction n.
-  - now unfold church_nat_aux.
-  - unfold church_nat_aux; fold church_nat_aux.
-    now unfold abstractionless; fold abstractionless.
-Qed. *)
-
-Compute let n:=2 in (increase_free_variables (church_nat_aux n) 2 2, church_nat_aux n).
-
-Lemma aux (n: nat): increase_free_variables (church_nat_aux n) 2 2 = church_nat_aux n.
+Lemma aux (n: nat): increase_free_variables (encode_aux n) 2 2 = encode_aux n.
 Proof.
   induction n.
   - now simpl.
-  - unfold church_nat_aux; fold church_nat_aux.
+  - unfold encode_aux; fold encode_aux.
     simpl.
     now rewrite IHn.
 Qed.
 
 
-Lemma aux' (n: nat): increase_free_variables (church_nat_aux n) 1 2 = church_nat_aux n.
+Lemma aux' (n: nat): increase_free_variables (encode_aux n) 1 2 = encode_aux n.
 Proof.
   induction n.
   - now simpl.
-  - unfold church_nat_aux; fold church_nat_aux.
+  - unfold encode_aux; fold encode_aux.
     simpl.
     now rewrite IHn.
 Qed.
 
 
 
-Lemma aux'' (n: nat): increase_free_variables (church_nat_aux n) 0 2 = church_nat_aux n.
+Lemma aux'' (n: nat): increase_free_variables (encode_aux n) 0 2 = encode_aux n.
 Proof.
   induction n.
   - now simpl.
-  - unfold church_nat_aux; fold church_nat_aux.
+  - unfold encode_aux; fold encode_aux.
     simpl.
     now rewrite IHn.
 Qed.
@@ -149,40 +67,40 @@ Qed.
 
 Require Import Coq.Classes.Morphisms. (* to use f_equiv if necessary *)
 
-Compute (replace (church_nat_aux 0) (# 1) 1).
-Compute (replace (church_nat_aux 1) (# 1) 1).
-Compute (replace (church_nat_aux 2) (# 1) 1).
-Compute (replace (church_nat_aux 3) (# 1) 1).
+Compute (replace (encode_aux 0) (# 1) 1).
+Compute (replace (encode_aux 1) (# 1) 1).
+Compute (replace (encode_aux 2) (# 1) 1).
+Compute (replace (encode_aux 3) (# 1) 1).
 
-Lemma lemma_replace (n: nat): replace (replace (church_nat_aux n) (# 1) 1) (# 0) 0 = church_nat_aux n.
+Lemma lemma_replace (n: nat): replace (replace (encode_aux n) (# 1) 1) (# 0) 0 = encode_aux n.
 Proof.
   induction n.
   - easy.
-  - unfold church_nat_aux; fold church_nat_aux.
+  - unfold encode_aux; fold encode_aux.
     simpl.
     f_equal.
     apply IHn.
 Qed.
 
-Lemma church_succ_respects_nat (n: nat): $ church_succ (church_nat n) == church_nat (S n).
+Lemma succ_encode (n: nat): $ succ (encode n) == encode (S n).
 Proof.
-  unfold church_succ.
-  Compute beta ($ (\ (\ (\ $ (# 1) $ $ (# 2) (# 1) (# 0)))) (church_nat n)) (PRoot).
-  transitivity (\ (\ $ (# 1) $ $ (church_nat n) (# 1) (# 0))).
+  unfold succ.
+  Compute beta ($ (\ (\ (\ $ (# 1) $ $ (# 2) (# 1) (# 0)))) (encode n)) (PRoot).
+  transitivity (\ (\ $ (# 1) $ $ (encode n) (# 1) (# 0))).
   - apply CStep.
     exists PRoot.
     simpl.
-    unfold church_nat.
+    unfold encode.
     now rewrite (aux n).
-  - unfold church_nat.
-    unfold church_nat_aux; fold church_nat_aux.
+  - unfold encode.
+    unfold encode_aux; fold encode_aux.
     destruct n.
     + common_reduct.
-    + unfold church_nat_aux; fold church_nat_aux.
-      transitivity (\\ $ (#1) $ (\ $ (#2) (replace (church_nat_aux n0) (#1) 1)) (#0)).
+    + unfold encode_aux; fold encode_aux.
+      transitivity (\\ $ (#1) $ (\ $ (#2) (replace (encode_aux n) (#1) 1)) (#0)).
       * apply CStep.
         now exists (PAbs (PAbs (PRight (PLeft PRoot)))).
-      * transitivity (\ (\ $ (# 1) $ (# 1) (replace (replace (church_nat_aux n0) (# 1) 1) (# 0) 0))).
+      * transitivity (\ (\ $ (# 1) $ (# 1) (replace (replace (encode_aux n) (# 1) 1) (# 0) 0))).
         -- apply CStep.
            now exists (PAbs (PAbs (PRight PRoot))).
         -- now rewrite lemma_replace.
@@ -191,29 +109,23 @@ Qed.
 
 
 
-Lemma church_nat_inj: forall (n m: nat), church_nat n == church_nat m -> n = m.
+Lemma encode_inj: forall (n m: nat), encode n == encode m -> n = m.
 Proof.
   intros.
-  induction n0, m.
+  unfold encode in H.
+  induction n, m.
   - easy.
-  - unfold church_nat in H.
-    unfold church_nat_aux in H; fold church_nat_aux in H.
+  - unfold encode in H.
+    unfold encode_aux in H; fold encode_aux in H.
     Admitted.
 
-Lemma church_succ_inj: forall (x y: term_nat), ($ church_succ (t x)) == ($ church_succ (t y)) -> (t x) == (t y).
+Lemma succ_inj: forall (x y: nat), ($ succ (encode x)) == ($ succ (encode y)) -> (encode x) == (encode y).
 Proof.
-  (* TODO create a tactic to rewrite term_nats into church_nat n? *)
+  (* TODO create a tactic to rewrite term_nats into encode n? *)
   intros.
-  destruct x, y.
-  destruct n0, n1.
-  simpl.
-  rewrite e.
-  rewrite e0.
-  simpl in H.
-  rewrite e, e0 in H.
-  rewrite church_succ_respects_nat in H.
-  rewrite church_succ_respects_nat in H.
-  apply church_nat_inj in H.
+  rewrite succ_encode in H.
+  rewrite succ_encode in H.
+  apply encode_inj in H.
   injection H.
   intro.
   rewrite H0.
@@ -223,16 +135,12 @@ Qed.
 
 (* TODO explain possible pitfall: \ x == \ #0 f_equal x == #0 !!! out of context #0 is nothing *)
 
-Lemma succ_zero: forall (x: term_nat), ~(($ church_succ (t x)) == church_nat 0).
+Lemma succ_zero: forall (x: nat), ~(($ succ (encode x)) == encode 0).
 Proof.
   intro.
-  destruct x.
-  destruct n0.
-  simpl.
-  rewrite e.
-  rewrite church_succ_respects_nat.
+  rewrite succ_encode.
   intro.
-  now apply church_nat_inj in H.
+  now apply encode_inj in H.
 Qed.
 
 
@@ -240,228 +148,333 @@ Qed.
 (* ASK associativity is weird as hell, why does Coq want THOSE parentheses? *)
 (* Definition plus: term := \\\\ $ ($ #3 #1) $ $ #2 #1 #0. *)
 
-Definition plus: term := \\ $ $ (#1) church_succ (#0).
-Definition zero: term_nat := church_nat' 0.
+Definition plus: term := \\ $ $ (#1) succ (#0).
 
-(* Lemma add_nat: forall (x y: nat), $ $ plus (church_nat x) (church_nat y) == church_nat (x + y).
+
+(* Lemma add_nat: forall (x y: nat), $ $ plus (encode x) (encode y) == encode (x + y).
 Proof.
   intros.
   induction x.
   -  *)
 
 
-Lemma repl_lemma (n: nat): replace (church_nat_aux n) (church_nat 0) 2 = church_nat_aux n.
+
+Lemma repl_lemma' (n: nat) (p: term): replace (encode_aux n) p 3 = encode_aux n.
 Proof.
   induction n.
   - easy.
-  - unfold church_nat_aux; fold church_nat_aux.
-    simpl.
-    now rewrite IHn.
-Qed.
-
-Lemma repl_lemma' (n: nat): replace (church_nat_aux n) (\ (\ (\ $ (# 1) $ $ (# 2) (# 1) (# 0)))) 3 =
-church_nat_aux n.
-Proof.
-  induction n.
-  - easy.
-  - unfold church_nat_aux; fold church_nat_aux.
-    simpl.
-    now rewrite IHn.
-Qed.
-
-
-Lemma repl_lemma'' (n: nat): replace (church_nat_aux n) (\ (\ church_nat_aux 0)) 2 = church_nat_aux n.
-Proof.
-  induction n.
-  - easy.
-  - unfold church_nat_aux; fold church_nat_aux.
+  - unfold encode_aux; fold encode_aux.
     simpl.
     repeat f_equal.
-    unfold church_nat_aux in IHn at 2.
+    unfold encode_aux in IHn at 2.
     apply IHn.
 Qed.
 
-Lemma repl_lemma''' (n: nat): replace (church_nat_aux n) $ plus (\ (\ church_nat_aux 0)) 3 = church_nat_aux n.
+Lemma repl_lemma (n: nat) (p: term): replace (encode_aux n) (p) 2 = encode_aux n.
 Proof.
   induction n.
   - easy.
-  - unfold church_nat_aux; fold church_nat_aux.
+  - unfold encode_aux; fold encode_aux.
     simpl.
     repeat f_equal.
-    unfold church_nat_aux in IHn at 2.
+    unfold encode_aux in IHn at 2.
     apply IHn.
 Qed.
 
 
 
-Lemma zero_neutral: forall (n: nat), $ $ plus (church_nat n) (church_nat 0) == church_nat n.
+Lemma zero_neutral: forall (n: nat), $ $ plus (encode n) (encode 0) == encode n.
 Proof.
   intros.
-  induction n0.
+  induction n.
   - common_reduct.
-  - rewrite <- church_succ_respects_nat.
-    rewrite <- IHn0 at 2.
+  - rewrite <- succ_encode.
+    rewrite <- IHn at 2.
     unfold plus.
-    transitivity ($ (\ $ ($ ($ church_succ (church_nat n0)) church_succ) (# 0)) (church_nat 0));
+    transitivity ($ (\ $ ($ ($ succ (encode n)) succ) (# 0)) (encode 0));
     [ apply CStep;
       exists (PLeft (PRoot));
       simpl;
       repeat f_equiv;
-      unfold church_nat;
+      unfold encode;
       repeat f_equal;
       apply aux' | ].
-    transitivity ($ $ $ church_succ (church_nat n0) church_succ (church_nat 0));
+    transitivity ($ $ $ succ (encode n) succ (encode 0));
     [ apply CStep;
       exists PRoot;
       simpl;
       repeat f_equal;
-      unfold church_nat at 2;
+      unfold encode at 2;
       repeat f_equal;
       apply repl_lemma | ].
     symmetry.
-    transitivity ($ church_succ $ (\ $ $ (church_nat n0) church_succ (# 0)) (church_nat 0));
+    transitivity ($ succ $ (\ $ $ (encode n) succ (# 0)) (encode 0));
     [ apply CStep;
       exists (PRight (PLeft PRoot));
       simpl;
       repeat f_equal;
-      unfold church_nat;
+      unfold encode;
       repeat f_equal;
       apply aux' | ].
-    transitivity ($ church_succ $ $ (church_nat n0) church_succ (church_nat 0));
+    transitivity ($ succ $ $ (encode n) succ (encode 0));
     [ apply CStep;
       exists (PRight PRoot);
       simpl;
       repeat f_equal;
-      unfold church_nat;
+      unfold encode;
       repeat f_equal;
       apply repl_lemma | ].
-    unfold church_succ.
-    transitivity (\\ $ (# 1) $ $ ($ $ (church_nat n0) (\ (\ (\ $ (# 1) $ $ (# 2) (# 1) (# 0)))) (church_nat 0)) (# 1) (# 0));
+    unfold succ.
+    transitivity (\\ $ (# 1) $ $ ($ $ (encode n) (\ (\ (\ $ (# 1) $ $ (# 2) (# 1) (# 0)))) (encode 0)) (# 1) (# 0));
     [ apply CStep;
       exists PRoot;
       simpl;
       repeat f_equal;
-      unfold church_nat;
+      unfold encode;
       repeat f_equal;
       apply aux | ].
     symmetry.
-    transitivity ($ $ (\ (\ $ (# 1) $ $ (church_nat n0) (# 1) (# 0))) (\ (\ (\ $ (# 1) $ $ (# 2) (# 1) (# 0)))) (church_nat 0));
+    transitivity ($ $ (\ (\ $ (# 1) $ $ (encode n) (# 1) (# 0))) (\ (\ (\ $ (# 1) $ $ (# 2) (# 1) (# 0)))) (encode 0));
     [ apply CStep;
       exists (PLeft (PLeft PRoot));
       simpl;
       repeat f_equal;
-      unfold church_nat;
+      unfold encode;
       repeat f_equal;
       apply aux | ].
-    transitivity ($ ((\ $ ((\ (\ (\ $ (# 1) $ $ (# 2) (# 1) (# 0))))) $ $ (church_nat n0) ((\ (\ (\ $ (# 1) $ $ (# 2) (# 1) (# 0))))) (# 0))) (church_nat 0));
+    transitivity ($ ((\ $ ((\ (\ (\ $ (# 1) $ $ (# 2) (# 1) (# 0))))) $ $ (encode n) ((\ (\ (\ $ (# 1) $ $ (# 2) (# 1) (# 0))))) (# 0))) (encode 0));
     [ apply CStep;
       exists (PLeft PRoot);
       simpl;
       repeat f_equal;
-      unfold church_nat;
+      unfold encode;
       repeat f_equal;
       apply repl_lemma' | ].
-    transitivity (($ (\ (\ (\ $ (# 1) $ $ (# 2) (# 1) (# 0)))) $ $ (church_nat n0) (\ (\ (\ $ (# 1) $ $ (# 2) (# 1) (# 0)))) (church_nat 0)));
+    transitivity (($ (\ (\ (\ $ (# 1) $ $ (# 2) (# 1) (# 0)))) $ $ (encode n) (\ (\ (\ $ (# 1) $ $ (# 2) (# 1) (# 0)))) (encode 0)));
     [ apply CStep;
       exists PRoot;
       simpl;
       repeat f_equal;
-      unfold church_nat;
+      unfold encode;
       repeat f_equal;
-      apply repl_lemma'' | ].
-    transitivity (((\ (\ $ (# 1) $ $ ($ $ (church_nat n0) (\ (\ (\ $ (# 1) $ $ (# 2) (# 1) (# 0)))) (church_nat 0)) (# 1) (# 0)))));
+      apply repl_lemma | ].
+    transitivity (((\ (\ $ (# 1) $ $ ($ $ (encode n) (\ (\ (\ $ (# 1) $ $ (# 2) (# 1) (# 0)))) (encode 0)) (# 1) (# 0)))));
     [ apply CStep;
       exists PRoot;
       simpl;
       repeat f_equal;
-      unfold church_nat;
+      unfold encode;
       repeat f_equal;
       apply aux | ].
     reflexivity.
 Qed.
 
-Definition mult := \\$ $ (#1) ($ plus #0) (church_nat 0).
+Ltac step p rt := transitivity p;
+  [ apply CStep;
+    exists rt;
+    simpl;
+    repeat f_equal;
+    unfold encode;
+    repeat f_equal;
+    try apply repl_lemma;
+    try apply repl_lemma';
+    try apply aux;
+    try apply aux';
+    try apply aux'' | ].
 
-Lemma mult_nil (n: nat): $ $ mult (church_nat n) (church_nat 0) == church_nat 0.
+
+Lemma plus_succ (n m: nat): $ $ plus (encode n) ($ succ (encode m)) == $ succ $ $ plus (encode n) (encode m).
+Proof.
+  induction m.
+  - rewrite zero_neutral.
+    unfold plus.
+    step ($ ((\ $ $ (encode n) succ (# 0))) $ succ (encode 0)) (PLeft PRoot).
+    step (($ $ (encode n) succ ($ succ (encode 0)))) (PRoot).
+    induction n.
+    + common_reduct.
+    + rewrite <- succ_encode.
+      unfold succ at 1.
+      step ($ $ ((\ (\ $ (# 1) $ $ (encode n) (# 1) (# 0)))) succ $ succ (encode 0)) (PLeft (PLeft PRoot)).
+      step ($ ((\ $ succ $ $ (encode n) succ (# 0))) $ succ (encode 0)) (PLeft PRoot).
+      step (($ succ $ $ (encode n) succ $ succ (encode 0))) PRoot.
+      f_equiv.
+      apply IHn.
+  - rewrite <- succ_encode.
+    unfold plus at 1.
+    step ($ ((\ $ $ (encode n) succ (# 0))) $ succ $ succ (encode m)) (PLeft PRoot).
+    step (($ $ (encode n) succ ($ succ $ succ (encode m)))) (PRoot).
+    rewrite IHm.
+    clear IHm.
+    induction n.
+    + unfold encode at 1.
+      unfold encode_aux at 1.
+      step ($ (\ # 0) $ succ $ succ (encode m)) (PLeft PRoot).
+      step ($ succ $ succ (encode m)) (PRoot).
+      repeat f_equiv.
+      unfold plus, encode at 2.
+      symmetry.
+      step ($ ((\ $ $ (\ (\ encode_aux 0)) succ (# 0))) (encode m)) (PLeft PRoot).
+      step ((($ $ (\ (\ encode_aux 0)) succ (encode m))) ) (PRoot).
+      unfold encode_aux.
+      step ($ ((\ # 0)) (encode m)) (PLeft PRoot).
+      step (encode m) (PRoot).
+      reflexivity.
+    + rewrite <- succ_encode in *.
+      unfold succ at 1.
+      step ($ $ ((\ (\ $ (# 1) $ $ (encode n) (# 1) (# 0)))) succ $ succ $ succ (encode m)) (PLeft (PLeft PRoot)).
+      step ($ ((\ $ succ $ $ (encode n) succ (# 0))) $ succ $ succ (encode m)) (PLeft PRoot).
+      step (($ succ $ $ (encode n) succ ($ succ $ succ (encode m)))) (PRoot).
+      f_equiv.
+      transitivity ($ succ $ succ $ $ plus (encode n) (encode m)).
+      * apply IHn.
+      * f_equiv.
+        symmetry.
+        unfold plus at 1.
+        step ($ ((\ $ $ $ succ (encode n) succ (# 0))) (encode m)) (PLeft PRoot).
+        step (($ $ $ succ (encode n) succ (encode m))) PRoot.
+        unfold succ at 1.
+        step ($ $ ((\ (\ $ (# 1) $ $ ((encode n)) (# 1) (# 0)))) succ (encode m)) (PLeft (PLeft PRoot)).
+        step ($ ((\ $ succ $ $ (encode n) succ (# 0))) (encode m)) (PLeft PRoot).
+        step ($ succ $ $ (encode n) succ (encode m)) PRoot.
+        f_equiv.
+        symmetry.
+        unfold plus.
+        step ($ ((\ $ $ (encode n) succ (# 0))) (encode m)) (PLeft PRoot).
+        step ($ $ (encode n) succ (encode m)) PRoot.
+        reflexivity.
+Qed.
+
+Definition mult := \\$ $ (#1) ($ plus #0) (encode 0).
+
+Lemma mult_nil (n: nat): $ $ mult (encode n) (encode 0) == encode 0.
 Proof.
   unfold mult.
-  transitivity ($ ((\ $ $ ((church_nat n)) $ plus (# 0) (church_nat 0))) (church_nat 0));
+  transitivity ($ ((\ $ $ ((encode n)) $ plus (# 0) (encode 0))) (encode 0));
   [ apply CStep;
     exists (PLeft PRoot);
     simpl;
     repeat f_equal;
-    unfold church_nat;
+    unfold encode;
     repeat f_equal;
     apply aux' | ].
-  transitivity ((($ $ ((church_nat n)) $ plus (church_nat 0) (church_nat 0))));
+  transitivity ((($ $ ((encode n)) $ plus (encode 0) (encode 0))));
   [ apply CStep;
     exists (PRoot);
     simpl;
     repeat f_equal;
-    unfold church_nat;
+    unfold encode;
     repeat f_equal;
     apply repl_lemma | ].
   induction n.
   - common_reduct.
-  - rewrite <- church_succ_respects_nat.
-    unfold church_succ.
-    transitivity ($ $ ((\ (\ $ (# 1) $ $ ((church_nat n0)) (# 1) (# 0)))) $ plus (church_nat 0) (church_nat 0));
+  - rewrite <- succ_encode.
+    unfold succ.
+    transitivity ($ $ ((\ (\ $ (# 1) $ $ ((encode n)) (# 1) (# 0)))) $ plus (encode 0) (encode 0));
     [ apply CStep;
       exists (PLeft (PLeft PRoot));
       simpl;
       repeat f_equal;
-      unfold church_nat;
+      unfold encode;
       repeat f_equal;
       apply aux | ].
-    transitivity ($ ((\ $ ($ plus (church_nat 0)) $ $ (church_nat n0) ($ plus (church_nat 0)) (# 0))) (church_nat 0));
+    transitivity ($ ((\ $ ($ plus (encode 0)) $ $ (encode n) ($ plus (encode 0)) (# 0))) (encode 0));
     [ apply CStep;
       exists (PLeft (PRoot));
       simpl;
       repeat f_equal;
-      unfold church_nat;
+      unfold encode;
       repeat f_equal;
-      apply repl_lemma''' | ].
-    transitivity (($ $ plus (church_nat 0) $ $ (church_nat n0) $ plus (church_nat 0) ((church_nat 0))) );
+      apply repl_lemma' | ].
+    transitivity (($ $ plus (encode 0) $ $ (encode n) $ plus (encode 0) ((encode 0))) );
     [ apply CStep;
       exists ((PRoot));
       simpl;
       repeat f_equal;
-      unfold church_nat;
+      unfold encode;
       repeat f_equal;
       apply repl_lemma | ].
     unfold plus at 1.
-    transitivity ($ ((\ $ $ (church_nat 0) church_succ (# 0))) $ $ (church_nat n0) $ plus (church_nat 0) (church_nat 0));
+    transitivity ($ ((\ $ $ (encode 0) succ (# 0))) $ $ (encode n) $ plus (encode 0) (encode 0));
     [ apply CStep;
       exists (PLeft (PRoot));
       simpl;
       repeat f_equal;
-      unfold church_nat;
+      unfold encode;
       repeat f_equal;
       apply repl_lemma | ].
-    transitivity (($ $ (church_nat 0) church_succ ($ $ (church_nat n0) $ plus (church_nat 0) (church_nat 0))));
+    transitivity (($ $ (encode 0) succ ($ $ (encode n) $ plus (encode 0) (encode 0))));
     [ apply CStep;
       exists ((PRoot));
       simpl;
       repeat f_equal;
-      unfold church_nat;
+      unfold encode;
       repeat f_equal;
       apply aux'' | ].
-    unfold church_nat at 1.
-    unfold church_nat_aux.
-    transitivity ($ ((\ # 0)) $ $ (church_nat n0) $ plus (church_nat 0) (church_nat 0));
+    unfold encode at 1.
+    unfold encode_aux.
+    transitivity ($ ((\ # 0)) $ $ (encode n) $ plus (encode 0) (encode 0));
     [ apply CStep;
       exists (PLeft (PRoot));
       simpl;
       repeat f_equal;
-      unfold church_nat;
+      unfold encode;
       repeat f_equal | ].
-    transitivity ($ $ (church_nat n0) $ plus (church_nat 0) (church_nat 0));
+    transitivity ($ $ (encode n) $ plus (encode 0) (encode 0));
     [ apply CStep;
       exists ((PRoot));
       simpl;
       repeat f_equal;
-      unfold church_nat;
+      unfold encode;
       repeat f_equal;
       apply aux'' | ].
       apply IHn.
 Qed.
+
+
+Lemma mult_plus (n m: nat): $ $ mult (encode n) ($ succ (encode m)) == $ $ plus $ $ mult (encode n) (encode m) (encode n).
+Proof.
+  induction n, m.
+  - common_reduct.
+  - rewrite <- succ_encode.
+    unfold mult.
+    step ($ ((\ $ $ ((encode 0)) $ plus (# 0) (encode 0))) $ succ $ succ (encode m)) (PLeft PRoot).
+    step (($ $ (encode 0) $ plus ($ succ $ succ (encode m)) (encode 0))) PRoot.
+    unfold encode at 1.
+    simpl.
+    step ($ ((\ # 0)) (encode 0)) (PLeft PRoot).
+    step (encode 0) PRoot.
+    symmetry.
+    unfold plus at 1.
+    step ($ ((\ $ $ ($ $ (\ (\ $ $ (# 1) $ plus (# 0) (encode 0))) (encode 0) $ succ (encode m)) succ (# 0))) (encode 0)) (PLeft PRoot).
+    step (($ $ $ $ (\ (\ $ $ (# 1) $ plus (# 0) (encode 0))) (encode 0) $ succ (encode m) succ ((encode 0)))) PRoot.
+    step ($ $ $ ((\ $ $ (encode 0) $ plus (# 0) (encode 0))) $ succ (encode m) succ (encode 0)) (PLeft (PLeft (PLeft PRoot))).
+    step ($ $ ($ $ (encode 0) $ plus ($ succ (encode m)) (encode 0)) succ (encode 0)) (PLeft (PLeft PRoot)).
+    unfold encode at 1.
+    simpl.
+    step ($ $ $ ((\ # 0)) (encode 0) succ (encode 0)) (PLeft (PLeft (PLeft PRoot))).
+    step ($ $ (encode 0) succ (encode 0)) (PLeft (PLeft PRoot)).
+    unfold encode at 1.
+    simpl.
+    step ($ ((\ # 0)) (encode 0)) (PLeft PRoot).
+    step (encode 0) PRoot.
+    reflexivity.
+  - rewrite mult_nil.
+    rewrite mult_nil in IHn.
+    rewrite <- succ_encode.
+    rewrite plus_succ.
+    rewrite <- IHn.
+    unfold mult at 1.
+    step ($ ((\ $ $ $ succ (encode n) $ plus (# 0) (encode 0))) $ succ (encode 0)) (PLeft PRoot).
+    step (($ $ $ succ (encode n) $ plus ($ succ (encode 0)) (encode 0))) PRoot.
+    symmetry.
+    unfold mult at 1.
+    step ($ succ $ ((\ $ $ ((encode n)) $ plus (# 0) (encode 0))) $ succ (encode 0)) (PRight (PLeft PRoot)).
+    step ($ succ ($ $ (encode n) $ plus ($ succ (encode 0)) (encode 0))) (PRight PRoot).
+    symmetry.
+    (* unfold plus at 1.
+    step ($ $ $ succ (encode n) ((\ $ $ ($ succ (encode 0)) succ (# 0))) (encode 0)) (PLeft (PRight PRoot)). *)
+    unfold succ at 1.
+    step ($ $ ((\ (\ $ (# 1) $ $ ((encode n)) (# 1) (# 0)))) $ plus $ succ (encode 0) (encode 0)) (PLeft (PLeft PRoot)).
+    step ($ ((\ $ ($ plus $ succ (encode 0)) $ $ (encode n) ($ plus $ succ (encode 0)) (# 0))) (encode 0)) (PLeft PRoot).
+    step (( $ $ plus $ succ (encode 0) $ $ (encode n) $ plus $ succ (encode 0) (encode 0))) PRoot.
+Admitted.
